<?xml version="1.0"?>
<rdf:RDF xmlns="https://github.com/NIH-NICHD/Data-Linkage-Governance#"
     xml:base="https://github.com/NIH-NICHD/Data-Linkage-Governance"
     xmlns:owl="http://www.w3.org/2002/07/owl#"
     xmlns:rdf="http://www.w3.org/1999/02/22-rdf-syntax-ns#"
     xmlns:xml="http://www.w3.org/XML/1998/namespace"
     xmlns:xsd="http://www.w3.org/2001/XMLSchema#"
     xmlns:odrl="http://www.w3.org/ns/odrl/2/"
     xmlns:rdfs="http://www.w3.org/2000/01/rdf-schema#"
     xmlns:skos="http://www.w3.org/2004/02/skos/core#"
     xmlns:terms="http://purl.org/dc/terms/"
     xmlns:data_governance_odrl="https://github.com/NIH-NICHD/Data-Linkage-Governance/">
    <owl:Ontology rdf:about="https://github.com/NIH-NICHD/Data-Linkage-Governance">
        <owl:imports rdf:resource="https://www.w3.org/ns/odrl/2/ODRL22.rdf"/>
        <terms:license>Apache License, Version 2.0</terms:license>
        <rdfs:comment xml:lang="en">This ontology provides a profile for the ODRL 2.2 specification that is specific to data governance and management in the context of data linkage.</rdfs:comment>
    </owl:Ontology>
    


    <!-- 
    ///////////////////////////////////////////////////////////////////////////////////////
    //
    // Annotation properties
    //
    ///////////////////////////////////////////////////////////////////////////////////////
     -->

    


    <!-- http://purl.org/dc/terms/title -->

    <owl:AnnotationProperty rdf:about="http://purl.org/dc/terms/title">
        <rdfs:label>Title</rdfs:label>
        <rdfs:domain rdf:resource="http://www.w3.org/ns/odrl/2/Policy"/>
    </owl:AnnotationProperty>
    


    <!-- http://www.w3.org/2004/02/skos/core#note -->

    <owl:AnnotationProperty rdf:about="http://www.w3.org/2004/02/skos/core#note">
        <rdfs:label>Note</rdfs:label>
        <rdfs:domain rdf:resource="http://www.w3.org/ns/odrl/2/Policy"/>
        <rdfs:domain rdf:resource="http://www.w3.org/ns/odrl/2/Rule"/>
    </owl:AnnotationProperty>
    


    <!-- https://github.com/NIH-NICHD/Data-Linkage-Governance/metadata_creation_date -->

    <owl:AnnotationProperty rdf:about="https://github.com/NIH-NICHD/Data-Linkage-Governance/metadata_creation_date">
        <rdfs:label>Metadata Creation Date</rdfs:label>
        <rdfs:domain rdf:resource="http://www.w3.org/ns/odrl/2/Policy"/>
    </owl:AnnotationProperty>
    


    <!-- 
    ///////////////////////////////////////////////////////////////////////////////////////
    //
    // Classes
    //
    ///////////////////////////////////////////////////////////////////////////////////////
     -->

    


    <!-- https://github.com/NIH-NICHD/Data-Linkage-Governance/Consent -->

    <owl:Class rdf:about="https://github.com/NIH-NICHD/Data-Linkage-Governance/Consent">
        <rdfs:subClassOf rdf:resource="http://www.w3.org/ns/odrl/2/Policy"/>
        <rdfs:label>Consent</rdfs:label>
        <skos:definition>Consent by a patient to participation in a clinical study after achieving an understanding of the relevant medical facts and the risks involved.

[source: https://ncithesaurus.nci.nih.gov/ncitbrowser/ConceptReport.jsp?dictionary=NCI_Thesaurus&amp;ns=ncit&amp;code=C16735]</skos:definition>
        <odrl:profile>Data Governance</odrl:profile>
    </owl:Class>
    


    <!-- https://github.com/NIH-NICHD/Data-Linkage-Governance/DataUseAgreement -->

    <owl:Class rdf:about="https://github.com/NIH-NICHD/Data-Linkage-Governance/DataUseAgreement">
        <rdfs:subClassOf rdf:resource="http://www.w3.org/ns/odrl/2/Policy"/>
        <rdfs:label>Data Use Agreement</rdfs:label>
        <skos:definition>A Data Use Agreement (DUA) is a legal contract between the entity that owns access to a data source, typically a dataset or database, and a secondary entity that will receive the data, or a subset of it, for reuse. A DUA outlines terms and limitations on how the shared data can be used, and the secondary entity may need to meet certain criteria, such as their affiliated institution, their faculty status, and IRB approval for their research study. Examples of limitations include restricting access to the shared data, requiring that any research dissemination include citation of the data and its originating entity, requiring that data files are destroyed at the completion of research period, and restrictions on data use for commercial purposes. DUAs are frequently required for access to data that contain protected health information (PHI). 

[source: https://www.nnlm.gov/guides/data-glossary/data-use-agreement]</skos:definition>
        <odrl:profile>Data Goveranance</odrl:profile>
    </owl:Class>
    


    <!-- https://github.com/NIH-NICHD/Data-Linkage-Governance/Dataset -->

    <owl:Class rdf:about="https://github.com/NIH-NICHD/Data-Linkage-Governance/Dataset">
        <rdfs:subClassOf rdf:resource="http://www.w3.org/ns/odrl/2/Asset"/>
        <rdfs:label>Dataset</rdfs:label>
        <skos:definition>A collection of related data records.

[source: 
URL:https://ncithesaurus.nci.nih.gov/ncitbrowser/ConceptReport.jsp?dictionary=NCI_Thesaurus&amp;ns=ncit&amp;code=C47824]</skos:definition>
        <odrl:profile>Data Governance</odrl:profile>
    </owl:Class>
    


    <!-- 
    ///////////////////////////////////////////////////////////////////////////////////////
    //
    // Individuals
    //
    ///////////////////////////////////////////////////////////////////////////////////////
     -->

    


    <!-- https://github.com/NIH-NICHD/Data-Linkage-Governance/AcademicResearch -->

    <owl:NamedIndividual rdf:about="https://github.com/NIH-NICHD/Data-Linkage-Governance/AcademicResearch">
        <rdf:type rdf:resource="http://www.w3.org/2004/02/skos/core#Concept"/>
        <rdf:type rdf:resource="http://www.w3.org/ns/odrl/2/RightOperand"/>
        <rdfs:label>Academic Research</rdfs:label>
        <skos:definition>Purposes associated with conducting or assisting with research conducted in an academic context e.g. within universities</skos:definition>
        <skos:exactMatch>https://w3id.org/dpv#ResearchAndDevelopment</skos:exactMatch>
    </owl:NamedIndividual>
    


    <!-- https://github.com/NIH-NICHD/Data-Linkage-Governance/ApprovedPurpose -->

    <owl:NamedIndividual rdf:about="https://github.com/NIH-NICHD/Data-Linkage-Governance/ApprovedPurpose">
        <rdf:type rdf:resource="http://www.w3.org/2004/02/skos/core#Concept"/>
        <rdf:type rdf:resource="http://www.w3.org/ns/odrl/2/RightOperand"/>
        <rdfs:label>Approved Purpose</rdfs:label>
    </owl:NamedIndividual>
    


    <!-- https://github.com/NIH-NICHD/Data-Linkage-Governance/DataEnclave -->

    <owl:NamedIndividual rdf:about="https://github.com/NIH-NICHD/Data-Linkage-Governance/DataEnclave">
        <rdf:type rdf:resource="http://www.w3.org/2004/02/skos/core#Concept"/>
        <rdf:type rdf:resource="http://www.w3.org/ns/odrl/2/RightOperand"/>
        <rdfs:label>Data Enclave</rdfs:label>
        <skos:definition>Use of cryptographic methods to restrict access and execution to trusted parties and code within a dedicated execution environment</skos:definition>
        <skos:exactMatch>https://w3id.org/dpv#TrustedExecutionEnvironments</skos:exactMatch>
    </owl:NamedIndividual>
    


    <!-- https://github.com/NIH-NICHD/Data-Linkage-Governance/DataRequester -->

    <owl:NamedIndividual rdf:about="https://github.com/NIH-NICHD/Data-Linkage-Governance/DataRequester">
        <rdf:type rdf:resource="http://www.w3.org/2004/02/skos/core#Concept"/>
        <rdf:type rdf:resource="http://www.w3.org/ns/odrl/2/Party"/>
        <rdfs:label>Data Requester</rdfs:label>
    </owl:NamedIndividual>
    


    <!-- https://github.com/NIH-NICHD/Data-Linkage-Governance/DataSteeringCommittee -->

    <owl:NamedIndividual rdf:about="https://github.com/NIH-NICHD/Data-Linkage-Governance/DataSteeringCommittee">
        <rdf:type rdf:resource="http://www.w3.org/2004/02/skos/core#Concept"/>
        <rdf:type rdf:resource="http://www.w3.org/ns/odrl/2/Party"/>
        <rdfs:label>Data Steering Committee</rdfs:label>
    </owl:NamedIndividual>
    


    <!-- https://github.com/NIH-NICHD/Data-Linkage-Governance/DeidentificationMethod -->

    <owl:NamedIndividual rdf:about="https://github.com/NIH-NICHD/Data-Linkage-Governance/DeidentificationMethod">
        <rdf:type rdf:resource="http://www.w3.org/2004/02/skos/core#Concept"/>
        <rdf:type rdf:resource="http://www.w3.org/ns/odrl/2/LeftOperand"/>
        <rdfs:label>Deidentification Method</rdfs:label>
    </owl:NamedIndividual>
    


    <!-- https://github.com/NIH-NICHD/Data-Linkage-Governance/LimitedDataSet -->

    <owl:NamedIndividual rdf:about="https://github.com/NIH-NICHD/Data-Linkage-Governance/LimitedDataSet">
        <rdf:type rdf:resource="http://www.w3.org/2004/02/skos/core#Concept"/>
        <rdf:type rdf:resource="http://www.w3.org/ns/odrl/2/RightOperand"/>
        <rdfs:label>Limited Data Set</rdfs:label>
    </owl:NamedIndividual>
    


    <!-- https://github.com/NIH-NICHD/Data-Linkage-Governance/SafeHarbor -->

    <owl:NamedIndividual rdf:about="https://github.com/NIH-NICHD/Data-Linkage-Governance/SafeHarbor">
        <rdf:type rdf:resource="http://www.w3.org/2004/02/skos/core#Concept"/>
        <rdf:type rdf:resource="http://www.w3.org/ns/odrl/2/RightOperand"/>
        <rdfs:label>Safe Harbor</rdfs:label>
    </owl:NamedIndividual>
    


    <!-- https://github.com/NIH-NICHD/Data-Linkage-Governance/StudySite -->

    <owl:NamedIndividual rdf:about="https://github.com/NIH-NICHD/Data-Linkage-Governance/StudySite">
        <rdf:type rdf:resource="http://www.w3.org/2004/02/skos/core#Concept"/>
        <rdf:type rdf:resource="http://www.w3.org/ns/odrl/2/Party"/>
        <rdfs:label>Study Site</rdfs:label>
    </owl:NamedIndividual>
    


    <!-- https://github.com/NIH-NICHD/Data-Linkage-Governance/access -->

    <owl:NamedIndividual rdf:about="https://github.com/NIH-NICHD/Data-Linkage-Governance/access">
        <rdf:type rdf:resource="http://www.w3.org/2004/02/skos/core#Concept"/>
        <rdf:type rdf:resource="http://www.w3.org/ns/odrl/2/Action"/>
        <odrl:includedIn rdf:resource="http://www.w3.org/ns/odrl/2/use"/>
        <rdfs:label>Access</rdfs:label>
        <skos:definition>To acquire data from a data repository or other data sharing system [NICHD ODSS]</skos:definition>
    </owl:NamedIndividual>
    


    <!-- https://github.com/NIH-NICHD/Data-Linkage-Governance/approve -->

    <owl:NamedIndividual rdf:about="https://github.com/NIH-NICHD/Data-Linkage-Governance/approve">
        <rdf:type rdf:resource="http://www.w3.org/2004/02/skos/core#Concept"/>
        <rdf:type rdf:resource="http://www.w3.org/ns/odrl/2/Action"/>
        <odrl:includedIn rdf:resource="http://www.w3.org/ns/odrl/2/use"/>
        <rdfs:label>Approve</rdfs:label>
        <skos:definition>To provide permission to perform data lifecycle activities, including collecting, linking, sharing, accessing, or using the data  [NICHD ODSS]</skos:definition>
    </owl:NamedIndividual>
    


    <!-- https://github.com/NIH-NICHD/Data-Linkage-Governance/classify -->

    <owl:NamedIndividual rdf:about="https://github.com/NIH-NICHD/Data-Linkage-Governance/classify">
        <rdf:type rdf:resource="http://www.w3.org/2004/02/skos/core#Concept"/>
        <rdf:type rdf:resource="http://www.w3.org/ns/odrl/2/Action"/>
        <odrl:includedIn rdf:resource="http://www.w3.org/ns/odrl/2/use"/>
        <rdfs:label>Classify</rdfs:label>
        <skos:definition>To organize data by relevant categories so that it may be used and protected more efficiently [DAMA-DMBOK]</skos:definition>
    </owl:NamedIndividual>
    


    <!-- https://github.com/NIH-NICHD/Data-Linkage-Governance/collect -->

    <owl:NamedIndividual rdf:about="https://github.com/NIH-NICHD/Data-Linkage-Governance/collect">
        <rdf:type rdf:resource="http://www.w3.org/2004/02/skos/core#Concept"/>
        <rdf:type rdf:resource="http://www.w3.org/ns/odrl/2/Action"/>
        <odrl:includedIn rdf:resource="http://www.w3.org/ns/odrl/2/use"/>
        <rdfs:label>Collect</rdfs:label>
        <skos:definition>To obtain data from participants for research, clinical, or administrative purposes [NICHD ODSS]</skos:definition>
    </owl:NamedIndividual>
    


    <!-- https://github.com/NIH-NICHD/Data-Linkage-Governance/completeTraining -->

    <owl:NamedIndividual rdf:about="https://github.com/NIH-NICHD/Data-Linkage-Governance/completeTraining">
        <rdf:type rdf:resource="http://www.w3.org/2004/02/skos/core#Concept"/>
        <rdf:type rdf:resource="http://www.w3.org/ns/odrl/2/Action"/>
        <odrl:includedIn rdf:resource="http://www.w3.org/ns/odrl/2/use"/>
        <rdfs:label>Complete Training</rdfs:label>
        <skos:definition>To complete training</skos:definition>
    </owl:NamedIndividual>
    


    <!-- https://github.com/NIH-NICHD/Data-Linkage-Governance/deidentify -->

    <owl:NamedIndividual rdf:about="https://github.com/NIH-NICHD/Data-Linkage-Governance/deidentify">
        <rdf:type rdf:resource="http://www.w3.org/2004/02/skos/core#Concept"/>
        <rdf:type rdf:resource="http://www.w3.org/ns/odrl/2/Action"/>
        <odrl:includedIn rdf:resource="http://www.w3.org/ns/odrl/2/use"/>
        <rdfs:label>Deidentify</rdfs:label>
        <skos:definition>To remove identifying information. De-identified patient data is patient information that has had personally identifiable information (PII; e.g. a person’s name, email address, or social security number), including protected health information (PHI; e.g. medical history, test results, and insurance information) removed. This is normally performed when sharing the data from a registry or clinical study to prevent a participant from being directly or indirectly identified. [NIH]</skos:definition>
    </owl:NamedIndividual>
    


    <!-- https://github.com/NIH-NICHD/Data-Linkage-Governance/link -->

    <owl:NamedIndividual rdf:about="https://github.com/NIH-NICHD/Data-Linkage-Governance/link">
        <rdf:type rdf:resource="http://www.w3.org/2004/02/skos/core#Concept"/>
        <rdf:type rdf:resource="http://www.w3.org/ns/odrl/2/Action"/>
        <odrl:implies rdf:resource="http://www.w3.org/ns/odrl/2/aggregate"/>
        <odrl:includedIn rdf:resource="http://www.w3.org/ns/odrl/2/use"/>
        <rdfs:label>Link</rdfs:label>
        <skos:definition>To combine information from a variety of data sources for the same individual [AHRQ] Synonymous with record linkage. [NICHD ODSS]</skos:definition>
    </owl:NamedIndividual>
    


    <!-- https://github.com/NIH-NICHD/Data-Linkage-Governance/makeDetermination -->

    <owl:NamedIndividual rdf:about="https://github.com/NIH-NICHD/Data-Linkage-Governance/makeDetermination">
        <rdf:type rdf:resource="http://www.w3.org/2004/02/skos/core#Concept"/>
        <rdf:type rdf:resource="http://www.w3.org/ns/odrl/2/Action"/>
        <odrl:includedIn rdf:resource="http://www.w3.org/ns/odrl/2/use"/>
        <rdfs:label>Make Determination</rdfs:label>
        <skos:definition>To reach a decision or draw conclusions for the purpose of data analysis</skos:definition>
    </owl:NamedIndividual>
    


    <!-- https://github.com/NIH-NICHD/Data-Linkage-Governance/obtainApproval -->

    <owl:NamedIndividual rdf:about="https://github.com/NIH-NICHD/Data-Linkage-Governance/obtainApproval">
        <rdf:type rdf:resource="http://www.w3.org/2004/02/skos/core#Concept"/>
        <rdf:type rdf:resource="http://www.w3.org/ns/odrl/2/Action"/>
        <odrl:includedIn rdf:resource="http://www.w3.org/ns/odrl/2/use"/>
        <rdfs:label>Obtain Approval</rdfs:label>
        <skos:definition>To obtain verifiable approval to perform the requested action in relation to the Asset.</skos:definition>
    </owl:NamedIndividual>
    


    <!-- https://github.com/NIH-NICHD/Data-Linkage-Governance/reidentify -->

    <owl:NamedIndividual rdf:about="https://github.com/NIH-NICHD/Data-Linkage-Governance/reidentify">
        <rdf:type rdf:resource="http://www.w3.org/2004/02/skos/core#Concept"/>
        <rdf:type rdf:resource="http://www.w3.org/ns/odrl/2/Action"/>
        <odrl:includedIn rdf:resource="http://www.w3.org/ns/odrl/2/use"/>
        <rdfs:label>Reidentify</rdfs:label>
        <skos:definition>To attribute information to de-identified data in order to identify the individual to whom the de-identified data relate [NIST]</skos:definition>
    </owl:NamedIndividual>
    


    <!-- https://github.com/NIH-NICHD/Data-Linkage-Governance/researchUse -->

    <owl:NamedIndividual rdf:about="https://github.com/NIH-NICHD/Data-Linkage-Governance/researchUse">
        <rdf:type rdf:resource="http://www.w3.org/2004/02/skos/core#Concept"/>
        <rdf:type rdf:resource="http://www.w3.org/ns/odrl/2/Action"/>
        <odrl:includedIn rdf:resource="http://www.w3.org/ns/odrl/2/use"/>
        <rdfs:label>Research Use</rdfs:label>
        <skos:definition>Working with data for secondary research or other analytical purposes [NICHD ODSS]</skos:definition>
    </owl:NamedIndividual>
    


    <!-- https://github.com/NIH-NICHD/Data-Linkage-Governance/secondaryLink -->

    <owl:NamedIndividual rdf:about="https://github.com/NIH-NICHD/Data-Linkage-Governance/secondaryLink">
        <rdf:type rdf:resource="http://www.w3.org/2004/02/skos/core#Concept"/>
        <rdf:type rdf:resource="http://www.w3.org/ns/odrl/2/Action"/>
        <odrl:includedIn rdf:resource="http://www.w3.org/ns/odrl/2/use"/>
        <rdfs:label>Secondary Link</rdfs:label>
        <skos:definition>To link a dataset for a secondary purpose distinct from the primary intended and approved purpose</skos:definition>
    </owl:NamedIndividual>
    


    <!-- https://github.com/NIH-NICHD/Data-Linkage-Governance/share -->

    <owl:NamedIndividual rdf:about="https://github.com/NIH-NICHD/Data-Linkage-Governance/share">
        <rdf:type rdf:resource="http://www.w3.org/2004/02/skos/core#Concept"/>
        <rdf:type rdf:resource="http://www.w3.org/ns/odrl/2/Action"/>
        <odrl:includedIn rdf:resource="http://www.w3.org/ns/odrl/2/use"/>
        <rdfs:label>Share</rdfs:label>
        <skos:definition>Making data available to the broader data user community, for example, by submitting the data to a data repository for dissemination [NICHD ODSS]</skos:definition>
    </owl:NamedIndividual>
    


    <!-- https://github.com/NIH-NICHD/Data-Linkage-Governance/sign -->

    <owl:NamedIndividual rdf:about="https://github.com/NIH-NICHD/Data-Linkage-Governance/sign">
        <rdf:type rdf:resource="http://www.w3.org/2004/02/skos/core#Concept"/>
        <rdf:type rdf:resource="http://www.w3.org/ns/odrl/2/Action"/>
        <odrl:includedIn rdf:resource="http://www.w3.org/ns/odrl/2/use"/>
        <rdfs:label>Sign</rdfs:label>
        <skos:definition>Signing a document or agreement</skos:definition>
    </owl:NamedIndividual>
    


    <!-- https://github.com/NIH-NICHD/Data-Linkage-Governance/submit -->

    <owl:NamedIndividual rdf:about="https://github.com/NIH-NICHD/Data-Linkage-Governance/submit">
        <rdf:type rdf:resource="http://www.w3.org/2004/02/skos/core#Concept"/>
        <rdf:type rdf:resource="http://www.w3.org/ns/odrl/2/Action"/>
        <odrl:includedIn rdf:resource="http://www.w3.org/ns/odrl/2/use"/>
        <rdfs:label>Submit</rdfs:label>
        <skos:definition>To submit a document such as a form, application, or protocol</skos:definition>
    </owl:NamedIndividual>
    


    <!-- 
    ///////////////////////////////////////////////////////////////////////////////////////
    //
    // Annotations
    //
    ///////////////////////////////////////////////////////////////////////////////////////
     -->

    <rdf:Description rdf:about="http://www.w3.org/ns/odrl/2/#constraintLeftOpCommon">
        <skos:member rdf:resource="https://github.com/NIH-NICHD/Data-Linkage-Governance/DeidentificationMethod"/>
    </rdf:Description>
    <rdf:Description rdf:about="http://www.w3.org/ns/odrl/2/#constraintRightOpCommon">
        <skos:member rdf:resource="https://github.com/NIH-NICHD/Data-Linkage-Governance/AcademicResearch"/>
        <skos:member rdf:resource="https://github.com/NIH-NICHD/Data-Linkage-Governance/ApprovedPurpose"/>
        <skos:member rdf:resource="https://github.com/NIH-NICHD/Data-Linkage-Governance/DataEnclave"/>
        <skos:member rdf:resource="https://github.com/NIH-NICHD/Data-Linkage-Governance/LimitedDataSet"/>
        <skos:member rdf:resource="https://github.com/NIH-NICHD/Data-Linkage-Governance/SafeHarbor"/>
    </rdf:Description>
    


    <!-- 
    ///////////////////////////////////////////////////////////////////////////////////////
    //
    // General axioms
    //
    ///////////////////////////////////////////////////////////////////////////////////////
     -->

    <rdf:Description>
        <rdf:type rdf:resource="http://www.w3.org/2002/07/owl#AllDisjointClasses"/>
        <owl:members rdf:parseType="Collection">
            <rdf:Description rdf:about="http://www.w3.org/ns/odrl/2/Agreement"/>
            <rdf:Description rdf:about="http://www.w3.org/ns/odrl/2/Assertion"/>
            <rdf:Description rdf:about="http://www.w3.org/ns/odrl/2/Offer"/>
            <rdf:Description rdf:about="http://www.w3.org/ns/odrl/2/Privacy"/>
            <rdf:Description rdf:about="http://www.w3.org/ns/odrl/2/Request"/>
            <rdf:Description rdf:about="http://www.w3.org/ns/odrl/2/Ticket"/>
            <rdf:Description rdf:about="https://github.com/NIH-NICHD/Data-Linkage-Governance/Consent"/>
            <rdf:Description rdf:about="https://github.com/NIH-NICHD/Data-Linkage-Governance/DataUseAgreement"/>
        </owl:members>
    </rdf:Description>
</rdf:RDF>



<!-- Generated by the OWL API (version 4.5.26.2023-07-17T20:34:13Z) https://github.com/owlcs/owlapi -->

