<?xml version="1.0"?>
<rdf:RDF xmlns="https://github.com/NIH-NICHD/Data-Linkage-Governance#"
     xml:base="https://github.com/NIH-NICHD/Data-Linkage-Governance"
     xmlns:owl="http://www.w3.org/2002/07/owl#"
     xmlns:rdf="http://www.w3.org/1999/02/22-rdf-syntax-ns#"
     xmlns:xml="http://www.w3.org/XML/1998/namespace"
     xmlns:xsd="http://www.w3.org/2001/XMLSchema#"
     xmlns:odrl="http://www.w3.org/ns/odrl/2/"
     xmlns:rdfs="http://www.w3.org/2000/01/rdf-schema#"
     xmlns:skos="http://www.w3.org/2004/02/skos/core#"
     xmlns:terms="http://purl.org/dc/terms/"
     xmlns:data_governance_odrl="https://github.com/NIH-NICHD/Data-Linkage-Governance/">
    <owl:Ontology rdf:about="https://github.com/NIH-NICHD/Data-Linkage-Governance">
        <owl:imports rdf:resource="https://www.w3.org/ns/odrl/2/ODRL22.rdf"/>
        <terms:license>Apache License, Version 2.0</terms:license>
        <rdfs:comment>Copyright 2024 The MITRE Corporation</rdfs:comment>
        <rdfs:comment xml:lang="en">This ontology provides a profile for the ODRL 2.2 specification that is specific to data governance and management in the context of data linkage.</rdfs:comment>
    </owl:Ontology>
    


    <!-- 
    ///////////////////////////////////////////////////////////////////////////////////////
    //
    // Annotation properties
    //
    ///////////////////////////////////////////////////////////////////////////////////////
     -->

    


    <!-- http://purl.org/dc/terms/title -->

    <owl:AnnotationProperty rdf:about="http://purl.org/dc/terms/title">
        <rdfs:label>Title</rdfs:label>
        <rdfs:domain rdf:resource="http://www.w3.org/ns/odrl/2/Policy"/>
    </owl:AnnotationProperty>
    


    <!-- http://www.w3.org/2004/02/skos/core#note -->

    <owl:AnnotationProperty rdf:about="http://www.w3.org/2004/02/skos/core#note">
        <rdfs:label>Note</rdfs:label>
        <rdfs:domain rdf:resource="http://www.w3.org/ns/odrl/2/Policy"/>
        <rdfs:domain rdf:resource="http://www.w3.org/ns/odrl/2/Rule"/>
    </owl:AnnotationProperty>
    


    <!-- 
    ///////////////////////////////////////////////////////////////////////////////////////
    //
    // Object Properties
    //
    ///////////////////////////////////////////////////////////////////////////////////////
     -->

    


    <!-- https://github.com/NIH-NICHD/Data-Linkage-Governance/approvedParty -->

    <owl:ObjectProperty rdf:about="https://github.com/NIH-NICHD/Data-Linkage-Governance/approvedParty">
        <rdfs:subPropertyOf rdf:resource="http://www.w3.org/ns/odrl/2/function"/>
        <rdfs:label>Approved Party</rdfs:label>
        <skos:definition>The party receiving approval.</skos:definition>
    </owl:ObjectProperty>
    


    <!-- https://github.com/NIH-NICHD/Data-Linkage-Governance/approvingParty -->

    <owl:ObjectProperty rdf:about="https://github.com/NIH-NICHD/Data-Linkage-Governance/approvingParty">
        <rdfs:subPropertyOf rdf:resource="http://www.w3.org/ns/odrl/2/function"/>
        <rdfs:label>Approving Party</rdfs:label>
        <skos:definition>The party providing approval.</skos:definition>
    </owl:ObjectProperty>
    


    <!-- https://github.com/NIH-NICHD/Data-Linkage-Governance/data_sharing_method -->

    <owl:ObjectProperty rdf:about="https://github.com/NIH-NICHD/Data-Linkage-Governance/data_sharing_method">
        <rdfs:subPropertyOf rdf:resource="http://www.w3.org/ns/odrl/2/function"/>
        <rdfs:label>Data Sharing Method</rdfs:label>
        <skos:definition>Description of how data was shared during previous linkage projects.</skos:definition>
    </owl:ObjectProperty>
    


    <!-- https://github.com/NIH-NICHD/Data-Linkage-Governance/entity_resolver -->

    <owl:ObjectProperty rdf:about="https://github.com/NIH-NICHD/Data-Linkage-Governance/entity_resolver">
        <rdfs:subPropertyOf rdf:resource="http://www.w3.org/ns/odrl/2/function"/>
        <rdfs:label>Entity Resolver</rdfs:label>
        <skos:definition>Description of organization performing entity resolution. Entity Resolution is the process of finding non-identical duplicate records.</skos:definition>
    </owl:ObjectProperty>
    


    <!-- https://github.com/NIH-NICHD/Data-Linkage-Governance/performing_party -->

    <owl:ObjectProperty rdf:about="https://github.com/NIH-NICHD/Data-Linkage-Governance/performing_party">
        <rdfs:subPropertyOf rdf:resource="http://www.w3.org/ns/odrl/2/function"/>
        <rdfs:label>Performing Party</rdfs:label>
        <skos:definition>Description of organization performing linkage.</skos:definition>
    </owl:ObjectProperty>
    


    <!-- https://github.com/NIH-NICHD/Data-Linkage-Governance/quality_assessment -->

    <owl:ObjectProperty rdf:about="https://github.com/NIH-NICHD/Data-Linkage-Governance/quality_assessment">
        <rdfs:subPropertyOf rdf:resource="http://www.w3.org/ns/odrl/2/function"/>
        <rdfs:label>Quality Assessment</rdfs:label>
        <skos:definition>Methods and results from an assessment of linkage quality.</skos:definition>
    </owl:ObjectProperty>
    


    <!-- 
    ///////////////////////////////////////////////////////////////////////////////////////
    //
    // Individuals
    //
    ///////////////////////////////////////////////////////////////////////////////////////
     -->

    


    <!-- https://github.com/NIH-NICHD/Data-Linkage-Governance/DeviceIdentifiersAndSerialNumbers -->

    <owl:NamedIndividual rdf:about="https://github.com/NIH-NICHD/Data-Linkage-Governance/DeviceIdentifiersAndSerialNumbers">
        <rdf:type rdf:resource="http://www.w3.org/2004/02/skos/core#Concept"/>
        <rdfs:label>Device Identifiers and Serial Numbers</rdfs:label>
        <skos:definition>The presence of the personally identifiable information element of device identifiers and serial numbers.</skos:definition>
    </owl:NamedIndividual>
    


    <!-- https://github.com/NIH-NICHD/Data-Linkage-Governance/EmailAddresses -->

    <owl:NamedIndividual rdf:about="https://github.com/NIH-NICHD/Data-Linkage-Governance/EmailAddresses">
        <rdf:type rdf:resource="http://www.w3.org/2004/02/skos/core#Concept"/>
        <rdfs:label>Email Addresses</rdfs:label>
        <skos:definition>The presence of the personally identifiable information element of an email address.</skos:definition>
    </owl:NamedIndividual>
    


    <!-- https://github.com/NIH-NICHD/Data-Linkage-Governance/FaxNumbers -->

    <owl:NamedIndividual rdf:about="https://github.com/NIH-NICHD/Data-Linkage-Governance/FaxNumbers">
        <rdf:type rdf:resource="http://www.w3.org/2004/02/skos/core#Concept"/>
        <rdfs:label>Fax Numbers</rdfs:label>
        <skos:definition>The presence of the personally identifiable information element of a fax number.</skos:definition>
    </owl:NamedIndividual>
    


    <!-- https://github.com/NIH-NICHD/Data-Linkage-Governance/FullFacePhotosAndComparableImages -->

    <owl:NamedIndividual rdf:about="https://github.com/NIH-NICHD/Data-Linkage-Governance/FullFacePhotosAndComparableImages">
        <rdf:type rdf:resource="http://www.w3.org/2004/02/skos/core#Concept"/>
        <rdfs:label>Full Face Photos and Comparable Images</rdfs:label>
        <skos:definition>The presence of the personally identifiable information element of a full face photo or comparable image.</skos:definition>
    </owl:NamedIndividual>
    


    <!-- https://github.com/NIH-NICHD/Data-Linkage-Governance/GeographicData -->

    <owl:NamedIndividual rdf:about="https://github.com/NIH-NICHD/Data-Linkage-Governance/GeographicData">
        <rdf:type rdf:resource="http://www.w3.org/2004/02/skos/core#Concept"/>
        <rdfs:label>Geographic Data</rdfs:label>
        <skos:definition>The presence of the personally identifiable information elements of geographic data. Includes street address, city, state, zip code, or elements of a geocode.</skos:definition>
    </owl:NamedIndividual>
    


    <!-- https://github.com/NIH-NICHD/Data-Linkage-Governance/HealthPlanBeneficiaryNumbers -->

    <owl:NamedIndividual rdf:about="https://github.com/NIH-NICHD/Data-Linkage-Governance/HealthPlanBeneficiaryNumbers">
        <rdf:type rdf:resource="http://www.w3.org/2004/02/skos/core#Concept"/>
        <rdfs:label>Health Plan Beneficiary Numbers</rdfs:label>
        <skos:definition>The presence of the personally identifiable information element of a health plan beneficiary or member number.</skos:definition>
    </owl:NamedIndividual>
    


    <!-- https://github.com/NIH-NICHD/Data-Linkage-Governance/IPAddresses -->

    <owl:NamedIndividual rdf:about="https://github.com/NIH-NICHD/Data-Linkage-Governance/IPAddresses">
        <rdf:type rdf:resource="http://www.w3.org/2004/02/skos/core#Concept"/>
        <rdfs:label>IP Addresses</rdfs:label>
        <skos:definition>The presence of the personally identifiable information element of an IP address.</skos:definition>
    </owl:NamedIndividual>
    


    <!-- https://github.com/NIH-NICHD/Data-Linkage-Governance/IRB -->

    <owl:NamedIndividual rdf:about="https://github.com/NIH-NICHD/Data-Linkage-Governance/IRB">
        <rdf:type rdf:resource="http://www.w3.org/2004/02/skos/core#Concept"/>
        <rdf:type rdf:resource="http://www.w3.org/ns/odrl/2/Party"/>
        <rdfs:label>Institutional Review Board</rdfs:label>
        <skos:definition>An Institutional Review Board (IRB) is the institutional entity charged with providing ethical and regulatory oversight of research involving human subjects, typically at the site of the research study. (source: https://orwh.od.nih.gov/toolkit/human-subjects-protections/institutional-review-board)</skos:definition>
    </owl:NamedIndividual>
    


    <!-- https://github.com/NIH-NICHD/Data-Linkage-Governance/MedicalRecordNumbers -->

    <owl:NamedIndividual rdf:about="https://github.com/NIH-NICHD/Data-Linkage-Governance/MedicalRecordNumbers">
        <rdf:type rdf:resource="http://www.w3.org/2004/02/skos/core#Concept"/>
        <rdfs:label>Medical Record Numbers (MRNs)</rdfs:label>
        <skos:definition>The presence of the personally identifiable information element of a medical record number.</skos:definition>
    </owl:NamedIndividual>
    


    <!-- https://github.com/NIH-NICHD/Data-Linkage-Governance/Names -->

    <owl:NamedIndividual rdf:about="https://github.com/NIH-NICHD/Data-Linkage-Governance/Names">
        <rdf:type rdf:resource="http://www.w3.org/2004/02/skos/core#Concept"/>
        <rdfs:label>Names</rdfs:label>
        <skos:definition>The presence of the personally identifiable information element of a name. Includes first, middle, and last name.</skos:definition>
    </owl:NamedIndividual>
    


    <!-- https://github.com/NIH-NICHD/Data-Linkage-Governance/PIIElement -->

    <owl:NamedIndividual rdf:about="https://github.com/NIH-NICHD/Data-Linkage-Governance/PIIElement">
        <rdf:type rdf:resource="http://www.w3.org/2004/02/skos/core#Collection"/>
        <skos:member rdf:resource="https://github.com/NIH-NICHD/Data-Linkage-Governance/DeviceIdentifiersAndSerialNumbers"/>
        <skos:member rdf:resource="https://github.com/NIH-NICHD/Data-Linkage-Governance/EmailAddresses"/>
        <skos:member rdf:resource="https://github.com/NIH-NICHD/Data-Linkage-Governance/FaxNumbers"/>
        <skos:member rdf:resource="https://github.com/NIH-NICHD/Data-Linkage-Governance/FullFacePhotosAndComparableImages"/>
        <skos:member rdf:resource="https://github.com/NIH-NICHD/Data-Linkage-Governance/GeographicData"/>
        <skos:member rdf:resource="https://github.com/NIH-NICHD/Data-Linkage-Governance/HealthPlanBeneficiaryNumbers"/>
        <skos:member rdf:resource="https://github.com/NIH-NICHD/Data-Linkage-Governance/IPAddresses"/>
        <skos:member rdf:resource="https://github.com/NIH-NICHD/Data-Linkage-Governance/MedicalRecordNumbers"/>
        <skos:member rdf:resource="https://github.com/NIH-NICHD/Data-Linkage-Governance/Names"/>
        <skos:member rdf:resource="https://github.com/NIH-NICHD/Data-Linkage-Governance/PhoneNumbers"/>
        <skos:member rdf:resource="https://github.com/NIH-NICHD/Data-Linkage-Governance/SocialSecurityNumbers"/>
        <skos:member rdf:resource="https://github.com/NIH-NICHD/Data-Linkage-Governance/URLs"/>
        <skos:member rdf:resource="https://github.com/NIH-NICHD/Data-Linkage-Governance/VehicleIdentifiersAndSerialNumbers"/>
        <skos:member rdf:resource="https://github.com/NIH-NICHD/Data-Linkage-Governance/accountNumbers"/>
        <skos:member rdf:resource="https://github.com/NIH-NICHD/Data-Linkage-Governance/anyOtherUniqueIdentifyingNumbersOrCodes"/>
        <skos:member rdf:resource="https://github.com/NIH-NICHD/Data-Linkage-Governance/biometricIdentifiers"/>
        <skos:member rdf:resource="https://github.com/NIH-NICHD/Data-Linkage-Governance/certificateLicenseNumbers"/>
        <skos:member rdf:resource="https://github.com/NIH-NICHD/Data-Linkage-Governance/dates"/>
    </owl:NamedIndividual>
    


    <!-- https://github.com/NIH-NICHD/Data-Linkage-Governance/PhoneNumbers -->

    <owl:NamedIndividual rdf:about="https://github.com/NIH-NICHD/Data-Linkage-Governance/PhoneNumbers">
        <rdf:type rdf:resource="http://www.w3.org/2004/02/skos/core#Concept"/>
        <rdfs:label>Phone Numbers</rdfs:label>
        <skos:definition>The presence of the personally identifiable information element of a phone number.</skos:definition>
    </owl:NamedIndividual>
    


    <!-- https://github.com/NIH-NICHD/Data-Linkage-Governance/PriorLinkage -->

    <owl:NamedIndividual rdf:about="https://github.com/NIH-NICHD/Data-Linkage-Governance/PriorLinkage">
        <rdf:type rdf:resource="http://www.w3.org/2004/02/skos/core#Concept"/>
        <rdfs:label>Prior Linkage</rdfs:label>
        <skos:definition>A set of information about prior linkages of a dataset.</skos:definition>
    </owl:NamedIndividual>
    


    <!-- https://github.com/NIH-NICHD/Data-Linkage-Governance/SocialSecurityNumbers -->

    <owl:NamedIndividual rdf:about="https://github.com/NIH-NICHD/Data-Linkage-Governance/SocialSecurityNumbers">
        <rdf:type rdf:resource="http://www.w3.org/2004/02/skos/core#Concept"/>
        <rdfs:label>Social Security Numbers (SSNs)</rdfs:label>
        <skos:definition>The presence of the personally identifiable information element of a social security number.</skos:definition>
    </owl:NamedIndividual>
    


    <!-- https://github.com/NIH-NICHD/Data-Linkage-Governance/URLs -->

    <owl:NamedIndividual rdf:about="https://github.com/NIH-NICHD/Data-Linkage-Governance/URLs">
        <rdf:type rdf:resource="http://www.w3.org/2004/02/skos/core#Concept"/>
        <rdfs:label>URLs</rdfs:label>
        <skos:definition>The presence of the personally identifiable information element of a URL.</skos:definition>
    </owl:NamedIndividual>
    


    <!-- https://github.com/NIH-NICHD/Data-Linkage-Governance/VehicleIdentifiersAndSerialNumbers -->

    <owl:NamedIndividual rdf:about="https://github.com/NIH-NICHD/Data-Linkage-Governance/VehicleIdentifiersAndSerialNumbers">
        <rdf:type rdf:resource="http://www.w3.org/2004/02/skos/core#Concept"/>
        <rdfs:label>Vehicle Identifiers and Serial Numbers</rdfs:label>
        <skos:definition>The presence of the personally identifiable information element of vehicle identifiers and serial numbers.</skos:definition>
    </owl:NamedIndividual>
    


    <!-- https://github.com/NIH-NICHD/Data-Linkage-Governance/academicResearch -->

    <owl:NamedIndividual rdf:about="https://github.com/NIH-NICHD/Data-Linkage-Governance/academicResearch">
        <rdf:type rdf:resource="http://www.w3.org/2004/02/skos/core#Concept"/>
        <rdf:type rdf:resource="http://www.w3.org/ns/odrl/2/RightOperand"/>
        <rdfs:label>Academic Research</rdfs:label>
        <skos:definition>Purposes associated with conducting or assisting with research conducted in an academic context e.g. within universities.</skos:definition>
    </owl:NamedIndividual>
    


    <!-- https://github.com/NIH-NICHD/Data-Linkage-Governance/access -->

    <owl:NamedIndividual rdf:about="https://github.com/NIH-NICHD/Data-Linkage-Governance/access">
        <rdf:type rdf:resource="http://www.w3.org/2004/02/skos/core#Concept"/>
        <rdf:type rdf:resource="http://www.w3.org/ns/odrl/2/Action"/>
        <odrl:includedIn rdf:resource="http://www.w3.org/ns/odrl/2/use"/>
        <rdfs:label>Access</rdfs:label>
        <skos:definition>To acquire data from a data repository or other data sharing system.</skos:definition>
        <skos:exactMatch>https://w3id.org/dpv#Access</skos:exactMatch>
    </owl:NamedIndividual>
    


    <!-- https://github.com/NIH-NICHD/Data-Linkage-Governance/accessType -->

    <owl:NamedIndividual rdf:about="https://github.com/NIH-NICHD/Data-Linkage-Governance/accessType">
        <rdf:type rdf:resource="http://www.w3.org/2004/02/skos/core#Concept"/>
        <rdf:type rdf:resource="http://www.w3.org/ns/odrl/2/LeftOperand"/>
        <rdfs:label>Access Type</rdfs:label>
        <skos:definition>The approach for making data available for use by others, for example open access or controlled access.</skos:definition>
    </owl:NamedIndividual>
    


    <!-- https://github.com/NIH-NICHD/Data-Linkage-Governance/accountNumbers -->

    <owl:NamedIndividual rdf:about="https://github.com/NIH-NICHD/Data-Linkage-Governance/accountNumbers">
        <rdf:type rdf:resource="http://www.w3.org/2004/02/skos/core#Concept"/>
        <rdfs:label>Account Numbers</rdfs:label>
        <skos:definition>The presence of the personally identifiable information element of an account number.</skos:definition>
    </owl:NamedIndividual>
    


    <!-- https://github.com/NIH-NICHD/Data-Linkage-Governance/anyOtherUniqueIdentifyingNumbersOrCodes -->

    <owl:NamedIndividual rdf:about="https://github.com/NIH-NICHD/Data-Linkage-Governance/anyOtherUniqueIdentifyingNumbersOrCodes">
        <rdf:type rdf:resource="http://www.w3.org/2004/02/skos/core#Concept"/>
        <rdfs:label>Any Other Unique Identifying Numbers or Codes</rdfs:label>
        <skos:definition>The presence of any other personally identifiable information elements.</skos:definition>
    </owl:NamedIndividual>
    


    <!-- https://github.com/NIH-NICHD/Data-Linkage-Governance/approve -->

    <owl:NamedIndividual rdf:about="https://github.com/NIH-NICHD/Data-Linkage-Governance/approve">
        <rdf:type rdf:resource="http://www.w3.org/2004/02/skos/core#Concept"/>
        <rdf:type rdf:resource="http://www.w3.org/ns/odrl/2/Action"/>
        <odrl:includedIn rdf:resource="http://www.w3.org/ns/odrl/2/use"/>
        <rdfs:label>Approve</rdfs:label>
        <skos:definition>To provide permission to perform data lifecycle activities, including collecting, linking, sharing, accessing, or using the data.</skos:definition>
        <skos:exactMatch>NCIt:C25425</skos:exactMatch>
    </owl:NamedIndividual>
    


    <!-- https://github.com/NIH-NICHD/Data-Linkage-Governance/approvedPurpose -->

    <owl:NamedIndividual rdf:about="https://github.com/NIH-NICHD/Data-Linkage-Governance/approvedPurpose">
        <rdf:type rdf:resource="http://www.w3.org/2004/02/skos/core#Concept"/>
        <rdf:type rdf:resource="http://www.w3.org/ns/odrl/2/RightOperand"/>
        <rdfs:label>Approved Purpose</rdfs:label>
        <skos:definition>The allowed activity or purpose for which the operator wishes to use the asset.</skos:definition>
    </owl:NamedIndividual>
    


    <!-- https://github.com/NIH-NICHD/Data-Linkage-Governance/biometricIdentifiers -->

    <owl:NamedIndividual rdf:about="https://github.com/NIH-NICHD/Data-Linkage-Governance/biometricIdentifiers">
        <rdf:type rdf:resource="http://www.w3.org/2004/02/skos/core#Concept"/>
        <rdfs:label>Biometric Identifiers</rdfs:label>
        <skos:definition>The presence of the personally identifiable information element of a biometric identifier.</skos:definition>
    </owl:NamedIndividual>
    


    <!-- https://github.com/NIH-NICHD/Data-Linkage-Governance/certificateLicenseNumbers -->

    <owl:NamedIndividual rdf:about="https://github.com/NIH-NICHD/Data-Linkage-Governance/certificateLicenseNumbers">
        <rdf:type rdf:resource="http://www.w3.org/2004/02/skos/core#Concept"/>
        <rdfs:label>Certificate License Numbers</rdfs:label>
        <skos:definition>The presence of the personally identifiable information element of a certificate license number.</skos:definition>
    </owl:NamedIndividual>
    


    <!-- https://github.com/NIH-NICHD/Data-Linkage-Governance/certification -->

    <owl:NamedIndividual rdf:about="https://github.com/NIH-NICHD/Data-Linkage-Governance/certification">
        <rdf:type rdf:resource="http://www.w3.org/2004/02/skos/core#Concept"/>
        <rdf:type rdf:resource="http://www.w3.org/ns/odrl/2/Agreement"/>
        <rdfs:label>Certification</rdfs:label>
        <skos:definition>An attestation that an official status has been earned by satisfying defined requirements, or the act of providing such a status, as proof that something has happened or defined standards have been met or will be upheld in the future.</skos:definition>
        <skos:exactMatch>https://w3id.org/dpv#Certification</skos:exactMatch>
    </owl:NamedIndividual>
    


    <!-- https://github.com/NIH-NICHD/Data-Linkage-Governance/certificationOrganization -->

    <owl:NamedIndividual rdf:about="https://github.com/NIH-NICHD/Data-Linkage-Governance/certificationOrganization">
        <rdf:type rdf:resource="http://www.w3.org/2004/02/skos/core#Concept"/>
        <rdf:type rdf:resource="http://www.w3.org/ns/odrl/2/Party"/>
        <rdfs:label>Certification Organization</rdfs:label>
        <skos:definition>An organization that grants or approves certifications or certificates.</skos:definition>
    </owl:NamedIndividual>
    


    <!-- https://github.com/NIH-NICHD/Data-Linkage-Governance/classify -->

    <owl:NamedIndividual rdf:about="https://github.com/NIH-NICHD/Data-Linkage-Governance/classify">
        <rdf:type rdf:resource="http://www.w3.org/2004/02/skos/core#Concept"/>
        <rdf:type rdf:resource="http://www.w3.org/ns/odrl/2/Action"/>
        <odrl:includedIn rdf:resource="http://www.w3.org/ns/odrl/2/use"/>
        <rdfs:label>Classify</rdfs:label>
        <skos:definition>To organize data by relevant categories so that it may be used and protected more efficiently.</skos:definition>
    </owl:NamedIndividual>
    


    <!-- https://github.com/NIH-NICHD/Data-Linkage-Governance/collect -->

    <owl:NamedIndividual rdf:about="https://github.com/NIH-NICHD/Data-Linkage-Governance/collect">
        <rdf:type rdf:resource="http://www.w3.org/2004/02/skos/core#Concept"/>
        <rdf:type rdf:resource="http://www.w3.org/ns/odrl/2/Action"/>
        <odrl:includedIn rdf:resource="http://www.w3.org/ns/odrl/2/use"/>
        <rdfs:label>Collect</rdfs:label>
        <skos:definition>The process of gathering and measuring information on variables of interest, in an established systematic fashion that enables one to answer stated research questions, test hypotheses, and evaluate outcomes.</skos:definition>
        <skos:exactMatch>https://w3id.org/dpv#Collect</skos:exactMatch>
    </owl:NamedIndividual>
    


    <!-- https://github.com/NIH-NICHD/Data-Linkage-Governance/completeTraining -->

    <owl:NamedIndividual rdf:about="https://github.com/NIH-NICHD/Data-Linkage-Governance/completeTraining">
        <rdf:type rdf:resource="http://www.w3.org/2004/02/skos/core#Concept"/>
        <rdf:type rdf:resource="http://www.w3.org/ns/odrl/2/Action"/>
        <odrl:includedIn rdf:resource="http://www.w3.org/ns/odrl/2/use"/>
        <rdfs:label>Complete Training</rdfs:label>
        <skos:definition>To complete training.</skos:definition>
    </owl:NamedIndividual>
    


    <!-- https://github.com/NIH-NICHD/Data-Linkage-Governance/consent -->

    <owl:NamedIndividual rdf:about="https://github.com/NIH-NICHD/Data-Linkage-Governance/consent">
        <rdf:type rdf:resource="http://www.w3.org/2004/02/skos/core#Concept"/>
        <rdf:type rdf:resource="http://www.w3.org/ns/odrl/2/Agreement"/>
        <rdfs:label>Consent</rdfs:label>
        <skos:definition>The IRB-approved written record that is in compliance with the Common Rule (45 CFR 46) and as applicable, Protection of Human Subjects rules (21 CFR 50), and is used to demonstrate the consent by a participant or guardian to participate in research.</skos:definition>
        <skos:exactMatch>https://w3id.org/dpv#Consent</skos:exactMatch>
    </owl:NamedIndividual>
    


    <!-- https://github.com/NIH-NICHD/Data-Linkage-Governance/consentRequirement -->

    <owl:NamedIndividual rdf:about="https://github.com/NIH-NICHD/Data-Linkage-Governance/consentRequirement">
        <rdf:type rdf:resource="http://www.w3.org/2004/02/skos/core#Concept"/>
        <rdf:type rdf:resource="http://www.w3.org/ns/odrl/2/LeftOperand"/>
        <rdfs:label>Consent Requirement</rdfs:label>
        <skos:definition>A requirement to obtain consent from a person or organization.</skos:definition>
    </owl:NamedIndividual>
    


    <!-- https://github.com/NIH-NICHD/Data-Linkage-Governance/contract -->

    <owl:NamedIndividual rdf:about="https://github.com/NIH-NICHD/Data-Linkage-Governance/contract">
        <rdf:type rdf:resource="http://www.w3.org/2004/02/skos/core#Concept"/>
        <rdf:type rdf:resource="http://www.w3.org/ns/odrl/2/Agreement"/>
        <rdfs:label>Contract</rdfs:label>
        <skos:definition>A contract is an agreement between parties, creating mutual obligations that are enforceable by law. (source: https://www.law.cornell.edu/wex/contract)</skos:definition>
        <skos:exactMatch>https://w3id.org/dpv#Contract</skos:exactMatch>
    </owl:NamedIndividual>
    


    <!-- https://github.com/NIH-NICHD/Data-Linkage-Governance/controlledAccess -->

    <owl:NamedIndividual rdf:about="https://github.com/NIH-NICHD/Data-Linkage-Governance/controlledAccess">
        <rdf:type rdf:resource="http://www.w3.org/2004/02/skos/core#Concept"/>
        <rdf:type rdf:resource="http://www.w3.org/ns/odrl/2/RightOperand"/>
        <rdfs:label>Controlled Access</rdfs:label>
        <skos:definition>Established processes for verifying appropriate use of shared data, such as requiring verification of requestor identity, committee approval of proposed research use, and signing a data use agreement to access protected data. (modified from source: https://grants.nih.gov/grants/guide/notice-files/NOT-OD-22-213.html)</skos:definition>
    </owl:NamedIndividual>
    


    <!-- https://github.com/NIH-NICHD/Data-Linkage-Governance/dataAccessCommittee -->

    <owl:NamedIndividual rdf:about="https://github.com/NIH-NICHD/Data-Linkage-Governance/dataAccessCommittee">
        <rdf:type rdf:resource="http://www.w3.org/2004/02/skos/core#Concept"/>
        <rdf:type rdf:resource="http://www.w3.org/ns/odrl/2/Party"/>
        <rdfs:label>Data Access Committee</rdfs:label>
        <skos:definition>A group of individuals who review all requests for access to datasets from external requestors and is composed of individuals with expertise in science, policy, or bioinformatics resources.</skos:definition>
    </owl:NamedIndividual>
    


    <!-- https://github.com/NIH-NICHD/Data-Linkage-Governance/dataCoordinatingCenter -->

    <owl:NamedIndividual rdf:about="https://github.com/NIH-NICHD/Data-Linkage-Governance/dataCoordinatingCenter">
        <rdf:type rdf:resource="http://www.w3.org/2004/02/skos/core#Concept"/>
        <rdf:type rdf:resource="http://www.w3.org/ns/odrl/2/Party"/>
        <rdfs:label>Data Coordinating Center</rdfs:label>
        <skos:definition>Academic and commercial data management and study oversight organizations, including contract research organizations, whose responsibilities include providing some or all the following services: study administration, financial management, protocol administration, data management, stakeholder communication and coordination, quality assurance, site monitoring, safety, regulatory, document management, post-study management, and close-out activities. (source:  https://www.niddk.nih.gov/-/media/Files/Research-Funding/Process/NIDDK-Guidance_DCC-Management-of-CCAs_Final_Version-1,-d-,1_OD-Approved_External-Website.pdf)</skos:definition>
    </owl:NamedIndividual>
    


    <!-- https://github.com/NIH-NICHD/Data-Linkage-Governance/dataEnclave -->

    <owl:NamedIndividual rdf:about="https://github.com/NIH-NICHD/Data-Linkage-Governance/dataEnclave">
        <rdf:type rdf:resource="http://www.w3.org/2004/02/skos/core#Concept"/>
        <rdf:type rdf:resource="http://www.w3.org/ns/odrl/2/RightOperand"/>
        <rdfs:label>Data Enclave</rdfs:label>
        <skos:definition>A secure network through which confidential data, such as identifiable information from census data, can be stored and disseminated. In a virtual data enclave a researcher can access the data from their own computer but cannot download or remove it from the remote server. Higher security data can be accessed through a physical data enclave where a researcher is required to access the data from a monitored room where the data is stored on non-network computers. (source: https://nnlm.gov/guides/data-thesaurus/data-enclave)</skos:definition>
        <skos:exactMatch>https://w3id.org/dpv#TrustedExecutionEnvironments</skos:exactMatch>
    </owl:NamedIndividual>
    


    <!-- https://github.com/NIH-NICHD/Data-Linkage-Governance/dataProvider -->

    <owl:NamedIndividual rdf:about="https://github.com/NIH-NICHD/Data-Linkage-Governance/dataProvider">
        <rdf:type rdf:resource="http://www.w3.org/2004/02/skos/core#Concept"/>
        <rdf:type rdf:resource="http://www.w3.org/ns/odrl/2/Party"/>
        <rdf:type rdf:resource="http://www.w3.org/ns/odrl/2/RightOperand"/>
        <rdfs:label>Data Provider</rdfs:label>
        <skos:definition>Institutions, organizations, and researchers that collect data from research participants or that collect administrative data and may also submit the data to a repository for sharing.</skos:definition>
    </owl:NamedIndividual>
    


    <!-- https://github.com/NIH-NICHD/Data-Linkage-Governance/dataRepository -->

    <owl:NamedIndividual rdf:about="https://github.com/NIH-NICHD/Data-Linkage-Governance/dataRepository">
        <rdf:type rdf:resource="http://www.w3.org/2004/02/skos/core#Concept"/>
        <rdf:type rdf:resource="http://www.w3.org/ns/odrl/2/Party"/>
        <rdfs:label>Data Repository</rdfs:label>
        <skos:definition>A physical location or virtual system for preserving, maintaining, and providing access to data. (modified from source: https://www.whitehouse.gov/wp-content/uploads/2022/05/05-2022-Desirable-Characteristics-of-Data-Repositories.pdf)</skos:definition>
    </owl:NamedIndividual>
    


    <!-- https://github.com/NIH-NICHD/Data-Linkage-Governance/dataRequester -->

    <owl:NamedIndividual rdf:about="https://github.com/NIH-NICHD/Data-Linkage-Governance/dataRequester">
        <rdf:type rdf:resource="http://www.w3.org/2004/02/skos/core#Concept"/>
        <rdf:type rdf:resource="http://www.w3.org/ns/odrl/2/LeftOperand"/>
        <rdf:type rdf:resource="http://www.w3.org/ns/odrl/2/Party"/>
        <rdfs:label>Data Requester</rdfs:label>
        <skos:definition>An individual or organization that requests access to a dataset that is not the participant.</skos:definition>
    </owl:NamedIndividual>
    


    <!-- https://github.com/NIH-NICHD/Data-Linkage-Governance/dataUseAgreement -->

    <owl:NamedIndividual rdf:about="https://github.com/NIH-NICHD/Data-Linkage-Governance/dataUseAgreement">
        <rdf:type rdf:resource="http://www.w3.org/2004/02/skos/core#Concept"/>
        <rdf:type rdf:resource="http://www.w3.org/ns/odrl/2/Agreement"/>
        <rdfs:label>Data Use Agreement</rdfs:label>
        <skos:definition>A document which establishes who is permitted to use and receive data, and the permitted uses and disclosures of such information by the recipient. (modified from source: https://www.hhs.gov/hipaa/for-professionals/special-topics/emergency-preparedness/data-use-agreement/index.html)</skos:definition>
    </owl:NamedIndividual>
    


    <!-- https://github.com/NIH-NICHD/Data-Linkage-Governance/dataset -->

    <owl:NamedIndividual rdf:about="https://github.com/NIH-NICHD/Data-Linkage-Governance/dataset">
        <rdf:type rdf:resource="http://www.w3.org/2004/02/skos/core#Concept"/>
        <rdf:type rdf:resource="http://www.w3.org/ns/odrl/2/Asset"/>
        <rdfs:label>Dataset</rdfs:label>
        <skos:definition>A collection of related data records.</skos:definition>
    </owl:NamedIndividual>
    


    <!-- https://github.com/NIH-NICHD/Data-Linkage-Governance/dates -->

    <owl:NamedIndividual rdf:about="https://github.com/NIH-NICHD/Data-Linkage-Governance/dates">
        <rdf:type rdf:resource="http://www.w3.org/2004/02/skos/core#Concept"/>
        <rdfs:label>Dates</rdfs:label>
        <skos:definition>The presence of the personally identifiable information element of dates. Includes birth dates and death dates.</skos:definition>
    </owl:NamedIndividual>
    


    <!-- https://github.com/NIH-NICHD/Data-Linkage-Governance/deidentificationMethod -->

    <owl:NamedIndividual rdf:about="https://github.com/NIH-NICHD/Data-Linkage-Governance/deidentificationMethod">
        <rdf:type rdf:resource="http://www.w3.org/2004/02/skos/core#Concept"/>
        <rdf:type rdf:resource="http://www.w3.org/ns/odrl/2/LeftOperand"/>
        <rdfs:label>Deidentification Method</rdfs:label>
        <skos:definition>The method to remove the identifiers or any information that could directly identify a participant from a dataset to mitigate privacy risks to that participant.</skos:definition>
    </owl:NamedIndividual>
    


    <!-- https://github.com/NIH-NICHD/Data-Linkage-Governance/deidentifiedDataset -->

    <owl:NamedIndividual rdf:about="https://github.com/NIH-NICHD/Data-Linkage-Governance/deidentifiedDataset">
        <rdf:type rdf:resource="http://www.w3.org/2004/02/skos/core#Concept"/>
        <rdf:type rdf:resource="http://www.w3.org/ns/odrl/2/RightOperand"/>
        <rdfs:label>Deidentified Dataset</rdfs:label>
        <skos:definition>A set of information that has had personally identifiable information (PII; e.g. a person’s name, email address, or social security number), including identifying protected health information (PHI; e.g., medical history, test results, and insurance information) removed.</skos:definition>
    </owl:NamedIndividual>
    


    <!-- https://github.com/NIH-NICHD/Data-Linkage-Governance/deidentify -->

    <owl:NamedIndividual rdf:about="https://github.com/NIH-NICHD/Data-Linkage-Governance/deidentify">
        <rdf:type rdf:resource="http://www.w3.org/2004/02/skos/core#Concept"/>
        <rdf:type rdf:resource="http://www.w3.org/ns/odrl/2/Action"/>
        <odrl:includedIn rdf:resource="http://www.w3.org/ns/odrl/2/use"/>
        <rdfs:label>Deidentify</rdfs:label>
        <skos:definition>To remove identifying information. De-identified data is participant information that has had personally identifiable information (PII; e.g. a participant’s name, email address, or social security number), including protected health information (PHI; e.g. medical history, test results, and insurance information) removed. This is normally performed when sharing the data from a registry or clinical study to prevent a participant from being directly or indirectly identified. (modified from source: https://toolkit.ncats.nih.gov/glossary/de-identified-patient-data/)</skos:definition>
    </owl:NamedIndividual>
    


    <!-- https://github.com/NIH-NICHD/Data-Linkage-Governance/determination -->

    <owl:NamedIndividual rdf:about="https://github.com/NIH-NICHD/Data-Linkage-Governance/determination">
        <rdf:type rdf:resource="http://www.w3.org/2004/02/skos/core#Concept"/>
        <rdf:type rdf:resource="http://www.w3.org/ns/odrl/2/Agreement"/>
        <rdfs:label>Determination</rdfs:label>
        <skos:definition>Outcome of a ruling or legal decision.</skos:definition>
    </owl:NamedIndividual>
    


    <!-- https://github.com/NIH-NICHD/Data-Linkage-Governance/disclosureReviewBody -->

    <owl:NamedIndividual rdf:about="https://github.com/NIH-NICHD/Data-Linkage-Governance/disclosureReviewBody">
        <rdf:type rdf:resource="http://www.w3.org/2004/02/skos/core#Concept"/>
        <rdf:type rdf:resource="http://www.w3.org/ns/odrl/2/Party"/>
        <rdfs:label>Disclosure Review Body</rdfs:label>
        <skos:definition>A group of individuals that establishes and operates processes and policies to ensure the public release of data products that do not reveal any information about the participants included in those datasets.</skos:definition>
    </owl:NamedIndividual>
    


    <!-- https://github.com/NIH-NICHD/Data-Linkage-Governance/governanceAction -->

    <owl:NamedIndividual rdf:about="https://github.com/NIH-NICHD/Data-Linkage-Governance/governanceAction">
        <rdf:type rdf:resource="http://www.w3.org/2004/02/skos/core#Collection"/>
        <skos:member rdf:resource="https://github.com/NIH-NICHD/Data-Linkage-Governance/access"/>
        <skos:member rdf:resource="https://github.com/NIH-NICHD/Data-Linkage-Governance/approve"/>
        <skos:member rdf:resource="https://github.com/NIH-NICHD/Data-Linkage-Governance/classify"/>
        <skos:member rdf:resource="https://github.com/NIH-NICHD/Data-Linkage-Governance/collect"/>
        <skos:member rdf:resource="https://github.com/NIH-NICHD/Data-Linkage-Governance/completeTraining"/>
        <skos:member rdf:resource="https://github.com/NIH-NICHD/Data-Linkage-Governance/deidentify"/>
        <skos:member rdf:resource="https://github.com/NIH-NICHD/Data-Linkage-Governance/link"/>
        <skos:member rdf:resource="https://github.com/NIH-NICHD/Data-Linkage-Governance/makeDetermination"/>
        <skos:member rdf:resource="https://github.com/NIH-NICHD/Data-Linkage-Governance/obtainApproval"/>
        <skos:member rdf:resource="https://github.com/NIH-NICHD/Data-Linkage-Governance/reidentify"/>
        <skos:member rdf:resource="https://github.com/NIH-NICHD/Data-Linkage-Governance/researchUse"/>
        <skos:member rdf:resource="https://github.com/NIH-NICHD/Data-Linkage-Governance/secondaryLink"/>
        <skos:member rdf:resource="https://github.com/NIH-NICHD/Data-Linkage-Governance/share"/>
        <skos:member rdf:resource="https://github.com/NIH-NICHD/Data-Linkage-Governance/sign"/>
        <skos:member rdf:resource="https://github.com/NIH-NICHD/Data-Linkage-Governance/submit"/>
    </owl:NamedIndividual>
    


    <!-- https://github.com/NIH-NICHD/Data-Linkage-Governance/governanceParty -->

    <owl:NamedIndividual rdf:about="https://github.com/NIH-NICHD/Data-Linkage-Governance/governanceParty">
        <rdf:type rdf:resource="http://www.w3.org/2004/02/skos/core#Collection"/>
        <skos:member rdf:resource="https://github.com/NIH-NICHD/Data-Linkage-Governance/IRB"/>
        <skos:member rdf:resource="https://github.com/NIH-NICHD/Data-Linkage-Governance/certificationOrganization"/>
        <skos:member rdf:resource="https://github.com/NIH-NICHD/Data-Linkage-Governance/dataAccessCommittee"/>
        <skos:member rdf:resource="https://github.com/NIH-NICHD/Data-Linkage-Governance/dataCoordinatingCenter"/>
        <skos:member rdf:resource="https://github.com/NIH-NICHD/Data-Linkage-Governance/dataProvider"/>
        <skos:member rdf:resource="https://github.com/NIH-NICHD/Data-Linkage-Governance/dataRepository"/>
        <skos:member rdf:resource="https://github.com/NIH-NICHD/Data-Linkage-Governance/dataRequester"/>
        <skos:member rdf:resource="https://github.com/NIH-NICHD/Data-Linkage-Governance/disclosureReviewBody"/>
        <skos:member rdf:resource="https://github.com/NIH-NICHD/Data-Linkage-Governance/governmentOrganization"/>
        <skos:member rdf:resource="https://github.com/NIH-NICHD/Data-Linkage-Governance/guardian"/>
        <skos:member rdf:resource="https://github.com/NIH-NICHD/Data-Linkage-Governance/participant"/>
        <skos:member rdf:resource="https://github.com/NIH-NICHD/Data-Linkage-Governance/principalInvestigator"/>
        <skos:member rdf:resource="https://github.com/NIH-NICHD/Data-Linkage-Governance/privacyBoard"/>
        <skos:member rdf:resource="https://github.com/NIH-NICHD/Data-Linkage-Governance/reviewCommittee"/>
    </owl:NamedIndividual>
    


    <!-- https://github.com/NIH-NICHD/Data-Linkage-Governance/governancePolicy -->

    <owl:NamedIndividual rdf:about="https://github.com/NIH-NICHD/Data-Linkage-Governance/governancePolicy">
        <rdf:type rdf:resource="http://www.w3.org/2004/02/skos/core#Collection"/>
        <skos:member rdf:resource="https://github.com/NIH-NICHD/Data-Linkage-Governance/certification"/>
        <skos:member rdf:resource="https://github.com/NIH-NICHD/Data-Linkage-Governance/consent"/>
        <skos:member rdf:resource="https://github.com/NIH-NICHD/Data-Linkage-Governance/contract"/>
        <skos:member rdf:resource="https://github.com/NIH-NICHD/Data-Linkage-Governance/dataUseAgreement"/>
        <skos:member rdf:resource="https://github.com/NIH-NICHD/Data-Linkage-Governance/determination"/>
        <skos:member rdf:resource="https://github.com/NIH-NICHD/Data-Linkage-Governance/law"/>
        <skos:member rdf:resource="https://github.com/NIH-NICHD/Data-Linkage-Governance/process"/>
    </owl:NamedIndividual>
    


    <!-- https://github.com/NIH-NICHD/Data-Linkage-Governance/governmentOrganization -->

    <owl:NamedIndividual rdf:about="https://github.com/NIH-NICHD/Data-Linkage-Governance/governmentOrganization">
        <rdf:type rdf:resource="http://www.w3.org/2004/02/skos/core#Concept"/>
        <rdf:type rdf:resource="http://www.w3.org/ns/odrl/2/Party"/>
        <rdfs:label>Government Organization</rdfs:label>
        <skos:definition>An international, federal, state, tribal, or local government organization. Inclusive of departments or divisions within a larger government organization.</skos:definition>
    </owl:NamedIndividual>
    


    <!-- https://github.com/NIH-NICHD/Data-Linkage-Governance/guardian -->

    <owl:NamedIndividual rdf:about="https://github.com/NIH-NICHD/Data-Linkage-Governance/guardian">
        <rdf:type rdf:resource="http://www.w3.org/2004/02/skos/core#Concept"/>
        <rdf:type rdf:resource="http://www.w3.org/ns/odrl/2/Party"/>
        <rdfs:label>Guardian</rdfs:label>
        <skos:definition>An individual who is authorized under applicable State or local law to consent on behalf of a child to general medical care. Inclusive of a child’s biological or adoptive parent. (source: https://www.ecfr.gov/current/title-45/subtitle-A/subchapter-A/part-46/subpart-D/section-46.402)</skos:definition>
    </owl:NamedIndividual>
    


    <!-- https://github.com/NIH-NICHD/Data-Linkage-Governance/law -->

    <owl:NamedIndividual rdf:about="https://github.com/NIH-NICHD/Data-Linkage-Governance/law">
        <rdf:type rdf:resource="http://www.w3.org/2004/02/skos/core#Concept"/>
        <rdf:type rdf:resource="http://www.w3.org/ns/odrl/2/Set"/>
        <rdfs:label>Law (regulations and statutes)</rdfs:label>
        <skos:definition>A system of rules created and enforced by governmental bodies that regulate the behavior of individuals, organizations, and governmental entities. Inclusive of statutes and regulations.</skos:definition>
        <skos:exactMatch>https://w3id.org/dpv#Law</skos:exactMatch>
    </owl:NamedIndividual>
    


    <!-- https://github.com/NIH-NICHD/Data-Linkage-Governance/limitedDataSet -->

    <owl:NamedIndividual rdf:about="https://github.com/NIH-NICHD/Data-Linkage-Governance/limitedDataSet">
        <rdf:type rdf:resource="http://www.w3.org/2004/02/skos/core#Concept"/>
        <rdf:type rdf:resource="http://www.w3.org/ns/odrl/2/RightOperand"/>
        <rdfs:label>Limited Dataset</rdfs:label>
        <skos:definition>A set of information about a participant that excludes 16 direct identifiers specified in the HIPAA Privacy Rule and may be used or disclosed, for purposes of research, public health, or health care operations, without obtaining either a participant&apos;s Authorization or a waiver or an alteration of authorization for its use and disclosure, with a data use agreement. (modified from source: https://privacyruleandresearch.nih.gov/pr_08.asp)</skos:definition>
    </owl:NamedIndividual>
    


    <!-- https://github.com/NIH-NICHD/Data-Linkage-Governance/link -->

    <owl:NamedIndividual rdf:about="https://github.com/NIH-NICHD/Data-Linkage-Governance/link">
        <rdf:type rdf:resource="http://www.w3.org/2004/02/skos/core#Concept"/>
        <rdf:type rdf:resource="http://www.w3.org/ns/odrl/2/Action"/>
        <odrl:implies rdf:resource="http://www.w3.org/ns/odrl/2/aggregate"/>
        <odrl:includedIn rdf:resource="http://www.w3.org/ns/odrl/2/use"/>
        <rdfs:label>Link</rdfs:label>
        <skos:definition>To combine information from a variety of data sources for the same participant. (source: https://hcup-us.ahrq.gov/datainnovations/raceethnicitytoolkit/or19.jsp) Synonymous with record linkage.</skos:definition>
    </owl:NamedIndividual>
    


    <!-- https://github.com/NIH-NICHD/Data-Linkage-Governance/linkageMethod -->

    <owl:NamedIndividual rdf:about="https://github.com/NIH-NICHD/Data-Linkage-Governance/linkageMethod">
        <rdf:type rdf:resource="http://www.w3.org/2004/02/skos/core#Concept"/>
        <rdf:type rdf:resource="http://www.w3.org/ns/odrl/2/LeftOperand"/>
        <rdfs:label>Linkage Method</rdfs:label>
        <skos:definition>The method used for linkage. Inclusive of PPRL and non-PPRL methods.</skos:definition>
    </owl:NamedIndividual>
    


    <!-- https://github.com/NIH-NICHD/Data-Linkage-Governance/makeDetermination -->

    <owl:NamedIndividual rdf:about="https://github.com/NIH-NICHD/Data-Linkage-Governance/makeDetermination">
        <rdf:type rdf:resource="http://www.w3.org/2004/02/skos/core#Concept"/>
        <rdf:type rdf:resource="http://www.w3.org/ns/odrl/2/Action"/>
        <odrl:includedIn rdf:resource="http://www.w3.org/ns/odrl/2/use"/>
        <rdfs:label>Make Determination</rdfs:label>
        <skos:definition>To reach a decision or draw conclusions.</skos:definition>
    </owl:NamedIndividual>
    


    <!-- https://github.com/NIH-NICHD/Data-Linkage-Governance/minorParticipant -->

    <owl:NamedIndividual rdf:about="https://github.com/NIH-NICHD/Data-Linkage-Governance/minorParticipant">
        <rdf:type rdf:resource="http://www.w3.org/2004/02/skos/core#Concept"/>
        <rdf:type rdf:resource="http://www.w3.org/ns/odrl/2/Party"/>
        <rdfs:label>Minor Participant</rdfs:label>
        <skos:definition>Refers to children or participants who have not attained the legal age for consent to treatments or procedures involved in the research, under the applicable law of the jurisdiction in which the research will be conducted. (modified from source: https://www.hhs.gov/ohrp/regulations-and-policy/guidance/faq/children-research/index.html)</skos:definition>
    </owl:NamedIndividual>
    


    <!-- https://github.com/NIH-NICHD/Data-Linkage-Governance/obtainApproval -->

    <owl:NamedIndividual rdf:about="https://github.com/NIH-NICHD/Data-Linkage-Governance/obtainApproval">
        <rdf:type rdf:resource="http://www.w3.org/2004/02/skos/core#Concept"/>
        <rdf:type rdf:resource="http://www.w3.org/ns/odrl/2/Action"/>
        <odrl:includedIn rdf:resource="http://www.w3.org/ns/odrl/2/use"/>
        <rdfs:label>Obtain Approval</rdfs:label>
        <skos:definition>To obtain verifiable approval to perform the requested action.</skos:definition>
    </owl:NamedIndividual>
    


    <!-- https://github.com/NIH-NICHD/Data-Linkage-Governance/output -->

    <owl:NamedIndividual rdf:about="https://github.com/NIH-NICHD/Data-Linkage-Governance/output">
        <rdf:type rdf:resource="http://www.w3.org/2004/02/skos/core#Concept"/>
        <rdf:type rdf:resource="http://www.w3.org/ns/odrl/2/LeftOperand"/>
        <rdfs:label>Output</rdfs:label>
        <skos:definition>The result of a process.</skos:definition>
    </owl:NamedIndividual>
    


    <!-- https://github.com/NIH-NICHD/Data-Linkage-Governance/participant -->

    <owl:NamedIndividual rdf:about="https://github.com/NIH-NICHD/Data-Linkage-Governance/participant">
        <rdf:type rdf:resource="http://www.w3.org/2004/02/skos/core#Concept"/>
        <rdf:type rdf:resource="http://www.w3.org/ns/odrl/2/Party"/>
        <rdfs:label>Participant</rdfs:label>
        <skos:definition>A healthy human or a patient who is or becomes a participant in research. (modified from source: https://policymanual.nih.gov/3014-001#C)</skos:definition>
        <skos:exactMatch>https://w3id.org/dpv#Participant</skos:exactMatch>
    </owl:NamedIndividual>
    


    <!-- https://github.com/NIH-NICHD/Data-Linkage-Governance/principalInvestigator -->

    <owl:NamedIndividual rdf:about="https://github.com/NIH-NICHD/Data-Linkage-Governance/principalInvestigator">
        <rdf:type rdf:resource="http://www.w3.org/2004/02/skos/core#Concept"/>
        <rdf:type rdf:resource="http://www.w3.org/ns/odrl/2/Party"/>
        <rdfs:label>Principal Investigator</rdfs:label>
        <skos:definition>The investigator with the overall responsibility for the designing, conducting, and reporting of the research, and must assure both the protocol and the research team’s actions are compliant with law, regulation, and NIH policy, even when certain aspects of the research are delegated to other investigators. (modified from source: https://ohsrp.nih.gov/confluence/display/ohsrp/Chapter+2+-+Roles+and+Responsibilities+of+the+Principal+Investigator#:~:text=The%20NIH%20Principal%20Investigator%20(PI,research%20to%20appropriately%20qualified%20individuals)</skos:definition>
    </owl:NamedIndividual>
    


    <!-- https://github.com/NIH-NICHD/Data-Linkage-Governance/privacyBoard -->

    <owl:NamedIndividual rdf:about="https://github.com/NIH-NICHD/Data-Linkage-Governance/privacyBoard">
        <rdf:type rdf:resource="http://www.w3.org/2004/02/skos/core#Concept"/>
        <rdf:type rdf:resource="http://www.w3.org/ns/odrl/2/Party"/>
        <rdfs:label>Privacy Board</rdfs:label>
        <skos:definition>A group of individuals who review and approve research uses and disclosures of data to ensure that the privacy rights of research participants are protected.</skos:definition>
    </owl:NamedIndividual>
    


    <!-- https://github.com/NIH-NICHD/Data-Linkage-Governance/process -->

    <owl:NamedIndividual rdf:about="https://github.com/NIH-NICHD/Data-Linkage-Governance/process">
        <rdf:type rdf:resource="http://www.w3.org/2004/02/skos/core#Concept"/>
        <rdf:type rdf:resource="http://www.w3.org/ns/odrl/2/Set"/>
        <rdfs:label>Process</rdfs:label>
        <skos:definition>A procedure that individuals are expected to adhere to or follow.</skos:definition>
        <skos:exactMatch>https://w3id.org/dpv#Process</skos:exactMatch>
    </owl:NamedIndividual>
    


    <!-- https://github.com/NIH-NICHD/Data-Linkage-Governance/reidentify -->

    <owl:NamedIndividual rdf:about="https://github.com/NIH-NICHD/Data-Linkage-Governance/reidentify">
        <rdf:type rdf:resource="http://www.w3.org/2004/02/skos/core#Concept"/>
        <rdf:type rdf:resource="http://www.w3.org/ns/odrl/2/Action"/>
        <odrl:includedIn rdf:resource="http://www.w3.org/ns/odrl/2/use"/>
        <rdfs:label>Reidentify</rdfs:label>
        <skos:definition>A general term for any process that re-establishes the relationship between identifying data and a participant. (modified from source: https://csrc.nist.gov/glossary/term/re_identification)</skos:definition>
    </owl:NamedIndividual>
    


    <!-- https://github.com/NIH-NICHD/Data-Linkage-Governance/researchUse -->

    <owl:NamedIndividual rdf:about="https://github.com/NIH-NICHD/Data-Linkage-Governance/researchUse">
        <rdf:type rdf:resource="http://www.w3.org/2004/02/skos/core#Concept"/>
        <rdf:type rdf:resource="http://www.w3.org/ns/odrl/2/Action"/>
        <odrl:includedIn rdf:resource="http://www.w3.org/ns/odrl/2/use"/>
        <rdfs:label>Research Use</rdfs:label>
        <skos:definition>Working with data for scientific research or other analytical purposes.</skos:definition>
    </owl:NamedIndividual>
    


    <!-- https://github.com/NIH-NICHD/Data-Linkage-Governance/reviewCommittee -->

    <owl:NamedIndividual rdf:about="https://github.com/NIH-NICHD/Data-Linkage-Governance/reviewCommittee">
        <rdf:type rdf:resource="http://www.w3.org/2004/02/skos/core#Concept"/>
        <rdf:type rdf:resource="http://www.w3.org/ns/odrl/2/Party"/>
        <rdfs:label>Review Committee</rdfs:label>
        <skos:definition>A group of individuals convened to review materials, provide approvals, and issue determinations on requested actions.</skos:definition>
    </owl:NamedIndividual>
    


    <!-- https://github.com/NIH-NICHD/Data-Linkage-Governance/safeHarborMethod -->

    <owl:NamedIndividual rdf:about="https://github.com/NIH-NICHD/Data-Linkage-Governance/safeHarborMethod">
        <rdf:type rdf:resource="http://www.w3.org/2004/02/skos/core#Concept"/>
        <rdf:type rdf:resource="http://www.w3.org/ns/odrl/2/RightOperand"/>
        <rdfs:label>Safe Harbor Method</rdfs:label>
        <skos:definition>A method for deidentification by removal of 18 HIPAA identifiers. (modified from source: https://www.hhs.gov/hipaa/for-professionals/privacy/special-topics/de-identification/index.html#safeharborguidance)</skos:definition>
    </owl:NamedIndividual>
    


    <!-- https://github.com/NIH-NICHD/Data-Linkage-Governance/secondaryLink -->

    <owl:NamedIndividual rdf:about="https://github.com/NIH-NICHD/Data-Linkage-Governance/secondaryLink">
        <rdf:type rdf:resource="http://www.w3.org/2004/02/skos/core#Concept"/>
        <rdf:type rdf:resource="http://www.w3.org/ns/odrl/2/Action"/>
        <odrl:includedIn rdf:resource="http://www.w3.org/ns/odrl/2/use"/>
        <rdfs:label>Secondary Link</rdfs:label>
        <skos:definition>To link a dataset for a secondary purpose distinct from the original or primary intended purpose.</skos:definition>
    </owl:NamedIndividual>
    


    <!-- https://github.com/NIH-NICHD/Data-Linkage-Governance/share -->

    <owl:NamedIndividual rdf:about="https://github.com/NIH-NICHD/Data-Linkage-Governance/share">
        <rdf:type rdf:resource="http://www.w3.org/2004/02/skos/core#Concept"/>
        <rdf:type rdf:resource="http://www.w3.org/ns/odrl/2/Action"/>
        <odrl:implies rdf:resource="http://creativecommons.org/ns#Sharing"/>
        <odrl:includedIn rdf:resource="http://www.w3.org/ns/odrl/2/use"/>
        <rdfs:label>Share</rdfs:label>
        <skos:definition>The act of making an asset such as a dataset available for use by others.</skos:definition>
    </owl:NamedIndividual>
    


    <!-- https://github.com/NIH-NICHD/Data-Linkage-Governance/sign -->

    <owl:NamedIndividual rdf:about="https://github.com/NIH-NICHD/Data-Linkage-Governance/sign">
        <rdf:type rdf:resource="http://www.w3.org/2004/02/skos/core#Concept"/>
        <rdf:type rdf:resource="http://www.w3.org/ns/odrl/2/Action"/>
        <odrl:includedIn rdf:resource="http://www.w3.org/ns/odrl/2/use"/>
        <rdfs:label>Sign</rdfs:label>
        <skos:definition>Signing a document or agreement.</skos:definition>
    </owl:NamedIndividual>
    


    <!-- https://github.com/NIH-NICHD/Data-Linkage-Governance/submit -->

    <owl:NamedIndividual rdf:about="https://github.com/NIH-NICHD/Data-Linkage-Governance/submit">
        <rdf:type rdf:resource="http://www.w3.org/2004/02/skos/core#Concept"/>
        <rdf:type rdf:resource="http://www.w3.org/ns/odrl/2/Action"/>
        <odrl:includedIn rdf:resource="http://www.w3.org/ns/odrl/2/use"/>
        <rdfs:label>Submit</rdfs:label>
        <skos:definition>To submit a document such as a form, application, or protocol.</skos:definition>
    </owl:NamedIndividual>
    


    <!-- 
    ///////////////////////////////////////////////////////////////////////////////////////
    //
    // Annotations
    //
    ///////////////////////////////////////////////////////////////////////////////////////
     -->

    <rdf:Description rdf:about="http://www.w3.org/ns/odrl/2/Policy">
        <skos:definition>A formal statement of intent or plan of action that is adopted by an organization  and defines specific procedures, rules, or regulations that individuals are expected to adhere to or follow.</skos:definition>
    </rdf:Description>
    <rdf:Description rdf:about="http://www.w3.org/ns/odrl/2/#constraintLeftOperandCommon">
        <skos:member rdf:resource="https://github.com/NIH-NICHD/Data-Linkage-Governance/accessType"/>
        <skos:member rdf:resource="https://github.com/NIH-NICHD/Data-Linkage-Governance/consentRequirement"/>
        <skos:member rdf:resource="https://github.com/NIH-NICHD/Data-Linkage-Governance/dataRequester"/>
        <skos:member rdf:resource="https://github.com/NIH-NICHD/Data-Linkage-Governance/deidentificationMethod"/>
        <skos:member rdf:resource="https://github.com/NIH-NICHD/Data-Linkage-Governance/linkageMethod"/>
        <skos:member rdf:resource="https://github.com/NIH-NICHD/Data-Linkage-Governance/output"/>
    </rdf:Description>
    <rdf:Description rdf:about="http://www.w3.org/ns/odrl/2/#constraintRightOpCommon">
        <skos:member rdf:resource="https://github.com/NIH-NICHD/Data-Linkage-Governance/AcademicResearch"/>
        <skos:member rdf:resource="https://github.com/NIH-NICHD/Data-Linkage-Governance/ApprovedPurpose"/>
        <skos:member rdf:resource="https://github.com/NIH-NICHD/Data-Linkage-Governance/ControlledAccess"/>
        <skos:member rdf:resource="https://github.com/NIH-NICHD/Data-Linkage-Governance/DataEnclave"/>
        <skos:member rdf:resource="https://github.com/NIH-NICHD/Data-Linkage-Governance/DeidentifiedDataset"/>
        <skos:member rdf:resource="https://github.com/NIH-NICHD/Data-Linkage-Governance/LimitedDataSet"/>
        <skos:member rdf:resource="https://github.com/NIH-NICHD/Data-Linkage-Governance/SafeHarborMethod"/>
        <skos:member rdf:resource="https://github.com/NIH-NICHD/Data-Linkage-Governance/dataProvider"/>
    </rdf:Description>
</rdf:RDF>



<!-- Generated by the OWL API (version 4.5.26.2023-07-17T20:34:13Z) https://github.com/owlcs/owlapi -->

